[optimizer] Define and certify a Michelson optimizer
The optimizer was initially designed for the backend of the Albert
compiler, it has been slightly generalized and certified. The main
theorem is the last one in file typed_optimizer.v:

If the untyped instruction sequence i can be typechecked from
stack type A to stack type B and then run successfully on stack
sA, then (optimizer.optimize i) can also be typechecked from
stack type A to stack type B and run successfully on stack sA
yielding the same result.

src/michocoq/error.v
@@ -97,6 +97,11 @@ Definition success {A} (m : M A) :=
   | Return _ => true
   end.
 
+Lemma bool_dec (b1 b2 : Datatypes.bool) : { b1 = b2 } + { b1 <> b2 }.
+Proof.
+  repeat decide equality.
+Qed.
+
 Definition Is_true := Bool.Is_true.
 
 Lemma Is_true_UIP b (x y : Is_true b) : x = y.
@@ -292,4 +297,38 @@ Proof.
   intro H.
   exists (existT_eq_1 P x y a b H).
   apply existT_eq_2.
+Defined.
+
+(* Same about sig *)
+
+Definition sig_eq_1 {A} (P : A -> Prop) (xa yb : sig P) : xa = yb -> proj1_sig xa = proj1_sig yb.
+Proof.
+  apply f_equal.
+Defined.
+
+Definition sig_eq_2 {A} (P : A -> Prop) (xa yb : sig P) (H : xa = yb) :
+  eq_rec (proj1_sig xa) P (proj2_sig xa) (proj1_sig yb) (sig_eq_1 P xa yb H) = proj2_sig yb.
+Proof.
+  subst xa.
+  reflexivity.
+Defined.
+
+Definition exist_eq_1 {A} (P : A -> Prop) x y a b : exist P x a = exist P y b -> x = y.
+Proof.
+  apply (f_equal (@proj1_sig A P)).
+Defined.
+
+Definition exist_eq_2 {A} (P : A -> Prop) x y a b (H : exist P x a = exist P y b ) :
+  eq_rec x P a y (exist_eq_1 P x y a b H) = b.
+Proof.
+  apply (sig_eq_2 P (exist P x a) (exist P y b)).
+Defined.
+
+Definition exist_eq_3 {A} (P : A -> Prop) x y a b :
+  exist P x a = exist P y b ->
+  sig (fun H : x = y => eq_rec x P a y H = b).
+Proof.
+  intro H.
+  exists (exist_eq_1 P x y a b H).
+  apply exist_eq_2.
 Defined.
