src/michocoq/optimizer.v
@@ -1,0 +1,108 @@
+(* Open Source License *)
+(* Copyright (c) 2019 Nomadic Labs. <contact@nomadic-labs.com> *)
+
+(* Permission is hereby granted, free of charge, to any person obtaining a *)
+(* copy of this software and associated documentation files (the "Software"), *)
+(* to deal in the Software without restriction, including without limitation *)
+(* the rights to use, copy, modify, merge, publish, distribute, sublicense, *)
+(* and/or sell copies of the Software, and to permit persons to whom the *)
+(* Software is furnished to do so, subject to the following conditions: *)
+
+(* The above copyright notice and this permission notice shall be included *)
+(* in all copies or substantial portions of the Software. *)
+
+(* THE SOFTWARE IS PROVIDED "AS IS", WITHOUT WARRANTY OF ANY KIND, EXPRESS OR *)
+(* IMPLIED, INCLUDING BUT NOT LIMITED TO THE WARRANTIES OF MERCHANTABILITY, *)
+(* FITNESS FOR A PARTICULAR PURPOSE AND NONINFRINGEMENT. IN NO EVENT SHALL *)
+(* THE AUTHORS OR COPYRIGHT HOLDERS BE LIABLE FOR ANY CLAIM, DAMAGES OR OTHER *)
+(* LIABILITY, WHETHER IN AN ACTION OF CONTRACT, TORT OR OTHERWISE, ARISING *)
+(* FROM, OUT OF OR IN CONNECTION WITH THE SOFTWARE OR THE USE OR OTHER *)
+(* DEALINGS IN THE SOFTWARE. *)
+
+(** Michelson optimizer working on the untyped syntax *)
+
+Require Import Michocoq.untyped_syntax.
+Require Import ZArith.
+
+(* Optimizations *)
+
+Fixpoint visit_instruction
+         (F : instruction_seq -> instruction_seq)
+         (i : instruction) {struct i} : instruction :=
+  match i with
+  | DIP n i => DIP n (visit_instruction_seq F i)
+  | IF_ f i1 i2 =>
+    IF_ f (visit_instruction_seq F i1) (visit_instruction_seq F i2)
+  | LOOP_ f i =>
+    LOOP_ f (visit_instruction_seq F i)
+  | ITER i => ITER (visit_instruction_seq F i)
+  | MAP i => MAP (visit_instruction_seq F i)
+  | LAMBDA a b i => LAMBDA a b i
+  | CREATE_CONTRACT a b an i => CREATE_CONTRACT a b an i
+  | PUSH ty x => PUSH ty x
+  | FAILWITH => FAILWITH
+  | SELF an => SELF an
+  | EXEC => EXEC
+  | instruction_opcode op => op
+  | Instruction_seq i =>
+    Instruction_seq (visit_instruction_seq F i)
+  end
+with
+visit_instruction_seq f i {struct i} :=
+  match i with
+  | NOOP => f NOOP
+  | SEQ i1 i2 =>
+    let i1' := visit_instruction f i1 in
+    let i2' := visit_instruction_seq f i2 in
+    f (SEQ i1' i2')
+  end.
+
+Definition dig0dug0 :=
+  visit_instruction_seq
+    (fun i =>
+       match i with
+       | SEQ (DIG 0) i => i
+       | SEQ (DUG 0) i => i
+       | SEQ (DROP 0) i => i
+       | SEQ (DIP 0 i1) i2 => instruction_app i1 i2
+       | SEQ (DIG 1) i => SEQ SWAP i
+       | SEQ (DUG 1) i => SEQ SWAP i
+       | SEQ (Instruction_seq i1) i2 => instruction_app i1 i2
+       | i => i
+       end).
+
+Definition digndugn :=
+  visit_instruction_seq
+    (fun i =>
+       match i with
+       | SEQ (DIG n1) (SEQ (DUG n2) i') =>
+         if (n1 =? n2) then i' else i
+       | i => i
+       end).
+
+Definition swapswap :=
+  visit_instruction_seq
+    (fun i =>
+       match i with
+       | SEQ SWAP (SEQ SWAP i) => i
+       | i => i
+       end).
+
+Definition push_drop :=
+  visit_instruction_seq
+    (fun i =>
+       match i with
+       | SEQ (PUSH _ _) (SEQ (DROP 1) i) => i
+       | SEQ (PUSH _ _) (SEQ (DROP (S n)) i) => SEQ (DROP n) i
+       | i => i
+       end).
+
+(** Clean some stuff in the code *)
+Definition cleanup (ins : instruction_seq) : instruction_seq :=
+  push_drop
+    (swapswap
+       (digndugn
+          (dig0dug0 ins))).
+
+(** Optimize the code (currently only cleanup of useless instructions *)
+Definition optimize := cleanup.
