src/michocoq/typed_optimizer.v
@@ -1,0 +1,1686 @@
+(* Open Source License *)
+(* Copyright (c) 2019 Nomadic Labs. <contact@nomadic-labs.com> *)
+
+(* Permission is hereby granted, free of charge, to any person obtaining a *)
+(* copy of this software and associated documentation files (the "Software"), *)
+(* to deal in the Software without restriction, including without limitation *)
+(* the rights to use, copy, modify, merge, publish, distribute, sublicense, *)
+(* and/or sell copies of the Software, and to permit persons to whom the *)
+(* Software is furnished to do so, subject to the following conditions: *)
+
+(* The above copyright notice and this permission notice shall be included *)
+(* in all copies or substantial portions of the Software. *)
+
+(* THE SOFTWARE IS PROVIDED "AS IS", WITHOUT WARRANTY OF ANY KIND, EXPRESS OR *)
+(* IMPLIED, INCLUDING BUT NOT LIMITED TO THE WARRANTIES OF MERCHANTABILITY, *)
+(* FITNESS FOR A PARTICULAR PURPOSE AND NONINFRINGEMENT. IN NO EVENT SHALL *)
+(* THE AUTHORS OR COPYRIGHT HOLDERS BE LIABLE FOR ANY CLAIM, DAMAGES OR OTHER *)
+(* LIABILITY, WHETHER IN AN ACTION OF CONTRACT, TORT OR OTHERWISE, ARISING *)
+(* FROM, OUT OF OR IN CONNECTION WITH THE SOFTWARE OR THE USE OR OTHER *)
+(* DEALINGS IN THE SOFTWARE. *)
+
+(* Same as the untyped optimizer but at the level of Michocoq.syntax *)
+
+From Michocoq Require untyped_syntax typer untyper.
+From Michocoq Require Import syntax.
+Import error.Notations.
+Import Notations.
+Require optimizer.
+Require Import ZArith.
+Require JMeq.
+Require Import String.
+
+Definition hide_tf {st A B} (i : instruction st true A B) :
+           sigT (fun tff => instruction st tff A B) :=
+  existT _ true i.
+
+Definition hide_ntf {st A B} (i : instruction st false A B) :
+           sigT (fun tff => instruction st tff A B) :=
+  existT _ false i.
+
+
+
+(* Manipulations of options *)
+
+Definition option_bind {A B}
+           (o : Datatypes.option A) (f : A -> Datatypes.option B) :
+  Datatypes.option B :=
+  match o with
+  | None => None
+  | Some a => f a
+  end.
+
+Notation "'let?' x ':=' X 'in' Y" :=
+  (option_bind X (fun x => Y))
+    (at level 200, x pattern, X at level 100, Y at level 200).
+
+Definition opt_get {A} (o : Datatypes.option A) (default : A) : A :=
+  match o with Some x => x | None => default end.
+
+Lemma unsome {A} (x y : A) : Some x = Some y -> x = y.
+Proof.
+  congruence.
+Qed.
+
+Lemma bind_some {A B} (y : Datatypes.option A) (w : B) z : (let? x := y in z x) = Some w <-> (exists x, y = Some x /\ z x = Some w).
+Proof.
+  destruct y; simpl; split.
+  - intro H; exists a; split; congruence.
+  - intros (x, (Hx, Hz)); congruence.
+  - discriminate.
+  - intros (x, (Hx, Hz)); discriminate.
+Qed.
+
+Fixpoint visit_instruction
+         (F : forall st tff A B,
+             instruction_seq st tff A B -> instruction_seq st tff A B)
+         {st tff A B}
+         (i : instruction st tff A B) {struct i} : instruction st tff A B :=
+  match i with
+  | Instruction_seq i => Instruction_seq (visit_instruction_seq F i)
+  | DIP n H i => DIP n H (visit_instruction_seq F i)
+  | IF_ f i1 i2 =>
+    IF_ f (visit_instruction_seq F i1) (visit_instruction_seq F i2)
+  | LOOP_ f i =>
+    LOOP_ f (visit_instruction_seq F i)
+  | ITER i => ITER (visit_instruction_seq F i)
+  | MAP i => MAP (visit_instruction_seq F i)
+
+  (* Note that LAMBDA a b i => LAMBDA a b (visit_instruction_seq F i)
+     would be incorrect because we can use PACK to distinguish
+     semantically equivalent lambdas in Michelson *)
+  | LAMBDA a b i => LAMBDA a b i
+  | CREATE_CONTRACT a b an i => CREATE_CONTRACT a b an i
+  | PUSH ty x => PUSH ty x
+  | FAILWITH => FAILWITH
+  | SELF an H => SELF an H
+  | EXEC => EXEC
+  | Instruction_opcode op => Instruction_opcode op
+  end
+with
+visit_instruction_seq f {st tff A B} (i : instruction_seq st tff A B) {struct i}
+: instruction_seq st tff A B :=
+  match i with
+  | NOOP => f _ _ _ _ NOOP
+  | Tail_fail i =>
+    let i' := visit_instruction f i in
+    f _ _ _ _ (Tail_fail i')
+  | SEQ i1 i2 =>
+    let i1' := visit_instruction f i1 in
+    let i2' := visit_instruction_seq f i2 in
+    f _ _ _ _ (SEQ i1' i2')
+  end.
+
+Definition untype_fun_seq
+           (F1 : forall st tff A B, instruction_seq st tff A B ->
+                                    instruction_seq st tff A B)
+           (F2 : untyped_syntax.instruction_seq -> untyped_syntax.instruction_seq) :=
+  forall st tff A B i,
+    untyper.untype_instruction_seq untyper.untype_Optimized (F1 st tff A B i) = F2 (untyper.untype_instruction_seq untyper.untype_Optimized i).
+
+Fixpoint untype_visit_instruction F1 F2
+         (H : untype_fun_seq F1 F2)
+         (HNOOP : F2 untyped_syntax.NOOP = untyped_syntax.NOOP)
+         st tff A B
+         (i : instruction st tff A B) :
+  untyper.untype_instruction untyper.untype_Optimized (visit_instruction F1 i) =
+  optimizer.visit_instruction F2 (untyper.untype_instruction untyper.untype_Optimized i)
+with
+untype_visit_instruction_seq F1 F2
+                             (H : untype_fun_seq F1 F2)
+                             (HNOOP : F2 untyped_syntax.NOOP = untyped_syntax.NOOP)
+                             st tff A B
+                             (i : instruction_seq st tff A B) :
+  untyper.untype_instruction_seq untyper.untype_Optimized (visit_instruction_seq F1 i) =
+  optimizer.visit_instruction_seq F2 (untyper.untype_instruction_seq  untyper.untype_Optimized i).
+Proof.
+  - destruct i; simpl; try reflexivity; try (repeat f_equal; apply untype_visit_instruction_seq; assumption).
+  - destruct i.
+    + apply H.
+    + simpl.
+      rewrite H.
+      simpl.
+      repeat f_equal.
+      * apply (untype_visit_instruction F1 F2); assumption.
+      * symmetry; assumption.
+    + simpl.
+      rewrite H.
+      simpl.
+      repeat f_equal.
+      * apply (untype_visit_instruction F1 F2); assumption.
+      * apply (untype_visit_instruction_seq F1 F2); assumption.
+Qed.
+
+Lemma stype_refl (A : Datatypes.list type) (H : A = A) : H = eq_refl.
+Proof.
+  apply Eqdep_dec.UIP_dec.
+  apply stype_dec.
+Qed.
+
+Lemma st_dec (st1 st2 : self_info) : sumbool (st1 = st2) (st1 <> st2).
+Proof.
+  repeat decide equality.
+Qed.
+
+Lemma st_refl (st : self_info) (H : st = st) : H = eq_refl.
+Proof.
+  apply Eqdep_dec.UIP_dec.
+  apply st_dec.
+Qed.
+
+Definition cast_instruction_seq_opt {st tff A B st' tff' A' B'}
+           (i : instruction_seq st tff A B)
+  : Datatypes.option (instruction_seq st' tff' A' B').
+Proof.
+  case (st_dec st st'); [| intros; exact None].
+  case (error.bool_dec tff tff'); [| intros; exact None].
+  case (stype_dec A A'); [| intros; exact None].
+  case (stype_dec B B'); [| intros; exact None].
+  intros; subst; exact (Some i).
+Defined.
+
+Lemma cast_instruction_seq_same {st tff A B} (i : instruction_seq st tff A B) :
+  cast_instruction_seq_opt i = Some i.
+Proof.
+  unfold cast_instruction_seq_opt.
+  destruct (st_dec st st) as [Hst | n]; [|destruct (n eq_refl)].
+  destruct (error.bool_dec tff tff) as [Htff | n]; [|destruct (n eq_refl)].
+  destruct (stype_dec A A) as [HA | n]; [|destruct (n eq_refl)].
+  destruct (stype_dec B B) as [HB | n]; [|destruct (n eq_refl)].
+  assert (HA = eq_refl) by apply stype_refl; subst.
+  assert (HB = eq_refl) by apply stype_refl; subst.
+  assert (Htff = eq_refl) by (apply Eqdep_dec.UIP_dec; apply error.bool_dec); subst.
+  assert (Hst = eq_refl) by apply st_refl; subst.
+  reflexivity.
+Qed.
+
+Definition dig0dug0_opt {st tff A C} (i : instruction_seq st tff A C) :
+  Datatypes.option (instruction_seq st tff A C)
+  :=
+  match i with
+  | Tail_fail i =>
+    let 'existT _ _ i := hide_tf i in
+    match i with
+    | Instruction_seq i => cast_instruction_seq_opt i
+    | _ => None
+    end
+  | @SEQ st' A' B _ _ i1 i2 =>
+    let 'existT _ _ i1 := hide_ntf i1 in
+    let? i1' :=
+       match i1 return Datatypes.option (instruction_seq st' false A' B) with
+       | DIP 0 _ i => cast_instruction_seq_opt i
+       | Instruction_seq i => cast_instruction_seq_opt i
+       | Instruction_opcode op =>
+         match op with
+         | @DIG _ 0 nil S2 a _ =>
+           cast_instruction_seq_opt (@NOOP st' (a ::: S2))
+         | @DUG _ 0 nil S2 a _ =>
+           cast_instruction_seq_opt (@NOOP st' (a ::: S2))
+         | @DIG _ 1 (cons a nil) S2 b _ =>
+           cast_instruction_seq_opt (SEQ (@SWAP st' a b S2) NOOP)
+         | @DUG _ 1 (cons a nil) S2 b _ =>
+           cast_instruction_seq_opt (SEQ (@SWAP st' b a S2) NOOP)
+         | @DROP _ 0 nil B' _ =>
+           cast_instruction_seq_opt (@NOOP st' B')
+         | _ => None
+         end
+       | _ => None
+       end in
+    cast_instruction_seq_opt (instruction_app i1' i2)
+  | _ => None
+  end.
+
+
+Inductive dig0dug0_opt_rel {st} :
+  forall {tff A B} (i i' : instruction_seq st tff A B), Prop :=
+| D0D0_tf A B (i : instruction_seq st true A B) :
+    dig0dug0_opt_rel (Tail_fail (Instruction_seq i)) i
+| D0D0_seq_is {tff A B C}
+              (i1 : instruction_seq st false A B)
+              (i2 : instruction_seq st tff B C) :
+    dig0dug0_opt_rel (SEQ (Instruction_seq i1) i2) (instruction_app i1 i2)
+| D0D0_DIP0 {tff A B C}
+            (i1 : instruction_seq st false A B)
+            (i2 : instruction_seq st tff B C) :
+    dig0dug0_opt_rel (SEQ (DIP (A := nil) 0 eq_refl i1) i2) (instruction_app i1 i2)
+| D0D0_DROP0 {tff A B}
+             (i : instruction_seq st tff A B) :
+    dig0dug0_opt_rel (SEQ (DROP (A := nil) 0 eq_refl) i) i
+| D0D0_DIG0 {tff t A B}
+            (i : instruction_seq st tff (t ::: A) B) :
+    dig0dug0_opt_rel (SEQ (DIG 0 (S1 := nil) eq_refl) i) i
+| D0D0_DUG0 {tff t A B}
+            (i : instruction_seq st tff (t ::: A) B) :
+    dig0dug0_opt_rel (SEQ (DUG 0 (S1 := nil) eq_refl) i) i
+| D0D0_DIG1 {tff a b A B}
+            (i : instruction_seq st tff (b ::: a ::: A) B) :
+    dig0dug0_opt_rel (SEQ (DIG 1 (S1 := _ ::: nil) eq_refl) i) (SEQ SWAP i)
+| D0D0_DUG1 {tff a b A B}
+            (i : instruction_seq st tff (b ::: a ::: A) B) :
+    dig0dug0_opt_rel (SEQ (DUG 1 (S1 := _ ::: nil) eq_refl) i) (SEQ SWAP i).
+
+Lemma uncons {A} (a1 a2 : A) l1 l2 :
+  cons a1 l1 = cons a2 l2 -> a1 = a2 /\ l1 = l2.
+Proof.
+  intro H; injection H; auto.
+Qed.
+
+Ltac destructable_list l :=
+  is_var l +
+  match l with
+  | nil => idtac
+  | cons _ _ => idtac
+  end.
+
+Ltac mytac :=
+  match goal with
+  | H : ?A |- _ =>
+    match A with
+    | existT _ _ _ = existT _ _ _ =>
+      apply error.existT_eq_3 in H
+    | exist _ _ _ = exist _ _ _ =>
+      apply error.exist_eq_3 in H
+    | hide_tf _ = existT _ _ _ =>
+      apply error.existT_eq_3 in H
+    | hide_ntf _ = existT _ _ _ =>
+      apply error.existT_eq_3 in H
+    | sig _ =>
+      destruct H
+    | sigT _ =>
+      destruct H
+    | exists _, _ =>
+      destruct H
+    | _ /\ _ =>
+      destruct H
+    | Datatypes.unit =>
+      destruct H
+    | eq_rec _ _ _ _ eq_refl = _ =>
+      simpl in H
+    | ?x = ?y =>
+      is_var x; subst x
+    | ?x = ?y =>
+      is_var y; subst y
+    | ?x = ?y =>
+      assert (H = eq_refl)
+        by (match type of x with
+            | Datatypes.bool => apply Eqdep_dec.UIP_refl_bool
+            | Datatypes.list type => apply Eqdep_dec.UIP_dec;
+                                     apply stype_dec
+            | type => apply Eqdep_dec.UIP_dec;
+                      apply type_dec
+            | Datatypes.nat => apply Eqdep_dec.UIP_dec;
+                               decide equality
+            end);
+      subst H
+    | cons ?a1 ?l1 = cons ?a2 ?l2 =>
+      (destructable_list l1 + destructable_list l2);
+      assert (a1 = a2 /\ l1 = l2) by (apply uncons; exact H)
+    | Some _ = Some _ =>
+      apply unsome in H
+    | Some _ = None => discriminate
+    | cast_instruction_seq_opt _ = _ =>
+      rewrite cast_instruction_seq_same in H
+    | option_bind (Some _) _ = _ =>
+      simpl in H
+    | option_bind None _ = _ =>
+      simpl in H
+    | option_bind _ _ = Some _ =>
+      apply bind_some in H
+    | option_bind (cast_instruction_seq_opt _) _ = _ =>
+      rewrite cast_instruction_seq_same in H
+    end
+  end.
+
+Lemma dig0dug0_opt_dig0dug0 {st tff A C} (i i' : instruction_seq st tff A C) :
+  dig0dug0_opt i = Some i' <-> dig0dug0_opt_rel i i'.
+Proof.
+  split.
+  - destruct i; try discriminate; unfold dig0dug0_opt.
+    + case_eq (hide_tf i).
+      intros tff i0 He Hi0.
+      destruct i0; try discriminate.
+      repeat mytac.
+      constructor.
+    + case_eq (hide_ntf i).
+      intros tff1 i1 He Hi1.
+      destruct i1; try discriminate.
+      * repeat mytac.
+        constructor.
+      * destruct n; try discriminate.
+        destruct A; try discriminate.
+        repeat mytac.
+        constructor.
+      * destruct o; try discriminate; destruct n as [|[|n]]; try discriminate.
+        -- destruct S1; try discriminate.
+           repeat mytac.
+           constructor.
+        -- destruct S1 as [|b [|]]; try discriminate.
+           repeat mytac.
+           constructor.
+        -- destruct S1; try discriminate.
+           repeat mytac.
+           constructor.
+        -- destruct S1 as [|b [|]]; try discriminate.
+           repeat mytac.
+           constructor.
+        -- destruct A; try discriminate.
+           repeat mytac.
+           constructor.
+  - intro Hi; destruct Hi; unfold dig0dug0_opt, hide_tf, hide_ntf;
+      repeat (rewrite cast_instruction_seq_same; simpl); reflexivity.
+Qed.
+
+Definition dig0dug0_aux {st tff A B} (i : instruction_seq st tff A B) : instruction_seq st tff A B :=
+  opt_get (dig0dug0_opt i) i.
+
+Definition dig0dug0 {st tff A B} (i : instruction_seq st tff A B) : instruction_seq st tff A B :=
+  visit_instruction_seq (@dig0dug0_aux) i.
+
+Lemma untyped_instruction_app_NOOP :
+  forall i, untyped_syntax.instruction_app i untyped_syntax.NOOP = i.
+Proof.
+  induction i.
+  - reflexivity.
+  - simpl; f_equal; assumption.
+Qed.
+
+Lemma untype_instruction_seq_app_aux {st tff1 tff2 A B C}
+         (i1 : instruction_seq st tff1 A B)
+         (i2 : instruction_seq st tff2 B C) H :
+  untyper.untype_instruction_seq untyper.untype_Optimized (instruction_app_aux i1 H  i2) =
+  untyped_syntax.instruction_app
+    (untyper.untype_instruction_seq untyper.untype_Optimized i1)
+    (untyper.untype_instruction_seq untyper.untype_Optimized i2).
+Proof.
+  induction i1; simpl.
+  - reflexivity.
+  - discriminate.
+  - f_equal.
+    apply IHi1.
+Qed.
+
+Lemma untype_instruction_seq_app {st tff A B C}
+         (i1 : instruction_seq st false A B)
+         (i2 : instruction_seq st tff B C) :
+  untyper.untype_instruction_seq untyper.untype_Optimized (i1;;; i2) =
+  untyped_syntax.instruction_app
+    (untyper.untype_instruction_seq untyper.untype_Optimized i1)
+    (untyper.untype_instruction_seq untyper.untype_Optimized i2).
+Proof.
+  apply untype_instruction_seq_app_aux.
+Qed.
+
+Lemma untype_dig0dug0 : untype_fun_seq (@dig0dug0) (optimizer.dig0dug0).
+Proof.
+  unfold untype_fun_seq, dig0dug0, optimizer.dig0dug0.
+  apply untype_visit_instruction_seq; [| reflexivity].
+  intros st tff A B i; simpl.
+  unfold dig0dug0_aux.
+  case_eq (dig0dug0_opt i).
+  - intros i' Hi.
+    apply dig0dug0_opt_dig0dug0 in Hi.
+    destruct Hi; simpl; try reflexivity;
+      try (symmetry; apply untyped_instruction_app_NOOP);
+      try apply untype_instruction_seq_app.
+  - intro HN.
+    simpl.
+    destruct i; try reflexivity.
+    + unfold dig0dug0_opt in HN.
+      case_eq (hide_tf i).
+      intros tff i' He.
+      rewrite He in HN.
+      destruct i'; try discriminate; repeat mytac; try reflexivity.
+      destruct tffa; try discriminate.
+      repeat mytac; simpl in *; repeat mytac; reflexivity.
+    + unfold dig0dug0_opt in HN.
+      case_eq (hide_ntf i).
+      intros tff1 i' He.
+      rewrite He in HN.
+      apply error.existT_eq_3 in He.
+      destruct He as (Htff', Hi).
+      destruct i'; try discriminate;
+        try (assert (Htff' = eq_refl) by apply Eqdep_dec.UIP_refl_bool;
+             subst Htff'; simpl in Hi; subst; reflexivity).
+      * repeat mytac.
+      * repeat mytac.
+        destruct tffa; simpl in *; repeat mytac; reflexivity.
+      * destruct n; destruct A as [|a A]; try discriminate; repeat mytac;
+          reflexivity.
+      * repeat mytac.
+        destruct o; try reflexivity.
+        -- destruct n as [|[|n]]; destruct S1 as [|a [|b S1]];
+             try discriminate; repeat mytac; reflexivity.
+        -- destruct n as [|[|n]]; destruct S1 as [|a [|b S1]];
+             try discriminate; repeat mytac; reflexivity.
+        -- destruct n as [|n]; destruct A as [|a A];
+             try discriminate; repeat mytac; reflexivity.
+Qed.
+
+(* Destructors for types instruction_seq, instruction, and opcode *)
+
+Definition unseq {st tff A C} (i : instruction_seq st tff A C):
+  Datatypes.option (sigT (fun B1 =>
+                            (sigT (fun B2 =>
+                                     instruction st false A B1 *
+                                     instruction_seq st tff B2 C))))%type :=
+  match i with
+  | NOOP => None
+  | Tail_fail _ => None
+  | SEQ i1 i2 =>
+    Some (existT _ _ (existT _ _ (i1, i2)))
+  end.
+
+Definition unseq_fst {st tff A C} (i : instruction_seq st tff A C):
+  Datatypes.option (sigT (fun A =>
+                            (sigT (fun B =>
+                                     instruction st false A B))))%type :=
+  match i with
+  | SEQ i1 i2 =>
+    Some (existT _ _ (existT _ _ i1))
+  | _ => None
+  end.
+
+Definition unseq_snd {st tff A C} (i : instruction_seq st tff A C):
+  Datatypes.option (sigT (fun B =>
+                            (sigT (fun C =>
+                                     instruction_seq st tff B C))))%type :=
+  match i with
+  | SEQ i1 i2 =>
+    Some (existT _ _ (existT _ _ i2))
+  | _ => None
+  end.
+
+Lemma unseq_seq {st tff A B C} (i : instruction_seq st tff A C) i1 i2 :
+  unseq i = Some (existT _ B (existT _ B (i1, i2))) <-> i = SEQ i1 i2.
+Proof.
+  split.
+  - destruct i; simpl; intro; try discriminate.
+    apply unsome in H.
+    apply error.existT_eq_3 in H.
+    destruct H as (He, H).
+    subst B0.
+    simpl in H.
+    apply error.existT_eq_3 in H.
+    destruct H as (He, H).
+    assert (He = eq_refl) by (apply Eqdep_dec.UIP_dec; apply stype_dec).
+    subst He.
+    simpl in H.
+    congruence.
+  - intro; subst i.
+    simpl.
+    reflexivity.
+Qed.
+
+Definition unopcode {st tff A B} (i : instruction st tff A B) :
+  Datatypes.option (@opcode st A B) :=
+  match i with
+  | Instruction_opcode op => Some op
+  | _ => None
+  end.
+
+Lemma unopcode_opcode {st tff A B} (i : instruction st tff A B) o (H : false = tff) :
+  unopcode i = Some o <->
+  i = eq_rec false (fun tff => instruction st tff A B) o tff H.
+Proof.
+  split.
+  - destruct i; simpl; intro; try discriminate.
+    apply unsome in H0.
+    subst o0.
+    assert (H = eq_refl) by apply Eqdep_dec.UIP_refl_bool.
+    subst H.
+    reflexivity.
+  - subst tff.
+    simpl.
+    intro; subst i.
+    reflexivity.
+Qed.
+
+Definition unswap_opcode {st A B} (op : @opcode st A B) : Datatypes.option Datatypes.unit :=
+  match op with
+  | SWAP => Some tt
+  | _ => None
+  end.
+
+Definition unswap {st tff A B} (i : instruction st tff A B) : Datatypes.option Datatypes.unit :=
+  let? op := unopcode i in unswap_opcode op.
+
+(* SWAP-SWAP *)
+
+Definition swapswap_opt {st tff A D} (i : instruction_seq st tff A D) :
+  Datatypes.option (instruction_seq st tff A D) :=
+  let? existT _ _ (existT _ _ i1) := unseq_fst i in
+  let? existT _ _ (existT _ _ i23) := unseq_snd i in
+  let '(existT _ _ i1) := hide_ntf i1 in
+  let? existT _ _ (existT _ _ i2) := unseq_fst i23 in
+  let '(existT _ _ i2) := hide_ntf i2 in
+  let? existT _ _ (existT _ _ i3) := unseq_snd i23 in
+  let? tt := unswap i1 in
+  let? tt := unswap i2 in
+  cast_instruction_seq_opt i3.
+
+Inductive swapswap_rel {st tff} :
+  forall {A B} (i i' : instruction_seq st tff A B), Prop :=
+| Swapswap_intro {a b A B} (i : instruction_seq st tff (a ::: b ::: A) B) :
+    swapswap_rel (SEQ SWAP (SEQ SWAP i)) i.
+
+Lemma swapswap_opt_swapswap {st tff A D} (i i' : instruction_seq st tff A D) :
+  swapswap_opt i = Some i' <-> swapswap_rel i i'.
+Proof.
+  split.
+  - unfold swapswap_opt.
+    intro H.
+    apply bind_some in H; destruct H as ((A1, (B1, i1)), (He1, H)).
+    apply bind_some in H; destruct H as ((A23, (B23, i23)), (He23, H)).
+    case_eq (hide_ntf i1); intros tff1 i1' Hi1'; rewrite Hi1' in H.
+    apply bind_some in H; destruct H as ((A2, (B2, i2)), (He2, H)).
+    case_eq (hide_ntf i2); intros tff2 i2' Hi2'; rewrite Hi2' in H.
+    apply bind_some in H; destruct H as ((A3, (B3, i3)), (He3, H)).
+
+    destruct i1'; try discriminate.
+    destruct o; try discriminate.
+    simpl in H.
+
+    destruct i2'; try discriminate.
+    destruct o; try discriminate.
+    simpl in H.
+
+    destruct i; try discriminate.
+    destruct i23; try discriminate.
+    simpl in *.
+    repeat mytac.
+    constructor.
+  - intro H.
+    destruct H.
+    simpl.
+    unfold swapswap_opt; simpl.
+    apply cast_instruction_seq_same.
+Qed.
+
+Definition swapswap_aux {st tff A D} (i : instruction_seq st tff A D) :
+  instruction_seq st tff A D :=
+  opt_get (swapswap_opt i) i.
+
+Definition swapswap {st tff A B} (i : instruction_seq st tff A B) : instruction_seq st tff A B :=
+  visit_instruction_seq (@swapswap_aux) i.
+
+Lemma untype_inversion_seq {st tff A C um} {i : instruction_seq st tff A C} {ui1 ui2} :
+  untyper.untype_instruction_seq um i = untyped_syntax.SEQ ui1 ui2 ->
+  (exists (H : tff = true) i',
+      eq_rec _ (fun tff => instruction_seq st tff A C) i _ H = Tail_fail i')
+  \/
+  (exists B (i1 : instruction st false A B) i2, i = SEQ i1 i2).
+Proof.
+  destruct i.
+  - discriminate.
+  - intro H; left.
+    exists eq_refl.
+    exists i.
+    reflexivity.
+  - intro H; right.
+    repeat eexists.
+Qed.
+
+Lemma untype_inversion_swap {st tff A B um} (i : instruction st tff A B) :
+  untyper.untype_instruction um i =
+  untyped_syntax.instruction_opcode untyped_syntax.SWAP ->
+  exists a b SA
+         (H : tff = false)
+         (HA : A = a ::: b ::: SA)
+         (HB : B = b ::: a ::: SA),
+    eq_rec
+      _
+      (fun A => instruction st false A (b ::: a ::: SA))
+      (eq_rec
+         _
+         (fun B => instruction st false A B)
+         (eq_rec _ (fun tff => instruction st tff A B) i _ H) _ HB) _ HA
+    = Instruction_opcode SWAP.
+Proof.
+  destruct i; try discriminate.
+  destruct o; try discriminate.
+  simpl.
+  intros _.
+  do 3 eexists.
+  do 3 (exists eq_refl).
+  reflexivity.
+Qed.
+
+Lemma untype_inversion_dig {st tff A B um} (i : instruction st tff A B) n :
+  untyper.untype_instruction um i =
+  untyped_syntax.instruction_opcode (untyped_syntax.DIG n) ->
+  exists S1 S2 t
+         (H : tff = false)
+         (HA : A = S1 +++ t ::: S2)
+         (HB : B = t ::: S1 +++ S2)
+         (Hn : n = List.length S1),
+    eq_rec
+      _
+      (fun A => instruction st false A (t ::: S1 +++ S2))
+      (eq_rec
+         _
+         (fun B => instruction st false A B)
+         (eq_rec _ (fun tff => instruction st tff A B) i _ H) _ HB) _ HA
+    = Instruction_opcode (@DIG _ (List.length S1) S1 S2 t eq_refl).
+Proof.
+  destruct i; try discriminate.
+  destruct o; try discriminate.
+  simpl.
+  intro H.
+  injection H.
+  intro; subst; clear H.
+  do 3 eexists.
+  do 4 (exists eq_refl).
+  reflexivity.
+Qed.
+
+Lemma untype_inversion_dug {st tff A B um} (i : instruction st tff A B) n :
+  untyper.untype_instruction um i =
+  untyped_syntax.instruction_opcode (untyped_syntax.DUG n) ->
+  exists S1 S2 t
+         (H : tff = false)
+         (HA : A = t ::: S1 +++ S2)
+         (HB : B = S1 +++ t ::: S2)
+         (Hn : n = List.length S1),
+    eq_rec
+      _
+      (fun A => instruction st false A (S1 +++ t ::: S2))
+      (eq_rec
+         _
+         (fun B => instruction st false A B)
+         (eq_rec _ (fun tff => instruction st tff A B) i _ H) _ HB) _ HA
+    = Instruction_opcode (@DUG _ (List.length S1) S1 S2 t eq_refl).
+Proof.
+  destruct i; try discriminate.
+  destruct o; try discriminate.
+  simpl.
+  intro H.
+  injection H.
+  intro; subst; clear H.
+  do 3 eexists.
+  do 4 (exists eq_refl).
+  reflexivity.
+Qed.
+
+Lemma untype_swapswap : untype_fun_seq (@swapswap) (optimizer.swapswap).
+Proof.
+  unfold untype_fun_seq, swapswap, optimizer.swapswap.
+  apply untype_visit_instruction_seq; [| reflexivity].
+  intros st tff A D i; simpl.
+  unfold swapswap_aux.
+  unfold opt_get.
+  case_eq (swapswap_opt i).
+  - intros i' H.
+    rewrite swapswap_opt_swapswap in H.
+    destruct H.
+    reflexivity.
+  - intro H.
+    unfold swapswap_opt in H.
+    case_eq (untyper.untype_instruction_seq untyper.untype_Optimized i);
+      try reflexivity.
+    intros ui1 ui23 Hi.
+    destruct ui1; try reflexivity.
+    destruct o; try reflexivity.
+    destruct ui23; try reflexivity.
+    destruct i0; try reflexivity.
+    destruct o; try reflexivity.
+    exfalso.
+    generalize (untype_inversion_seq Hi).
+    intro Hiinv.
+    destruct Hiinv as [(Htff, (i', Hi')) | (B, (i1, (i23, Hi123)))].
+    * repeat mytac.
+      discriminate.
+    * subst i.
+      simpl in Hi.
+      injection Hi.
+      intros Hi23 Hi1.
+      generalize (untype_inversion_seq Hi23).
+      intros Hiinv.
+      destruct Hiinv as [(Htff, (i', Hi')) | (C, (i2, (i3, Hi23')))].
+      -- repeat mytac.
+         injection Hi23.
+         intros Hui23 Hi'.
+         apply untype_inversion_swap in Hi'.
+         repeat mytac.
+         discriminate.
+      -- repeat mytac.
+         injection Hi23.
+         intros Hi3 Hi2.
+         apply untype_inversion_swap in Hi1.
+         apply untype_inversion_swap in Hi2.
+         repeat mytac.
+         simpl in H.
+         repeat mytac.
+Qed.
+
+(* DIG n - DUG n *)
+
+
+Definition undig_opcode {st A B} (op : @opcode st A B) : Datatypes.option Datatypes.nat :=
+  match op with
+  | DIG n _ => Some n
+  | _ => None
+  end.
+
+Definition undug_opcode {st A B} (op : @opcode st A B) : Datatypes.option Datatypes.nat :=
+  match op with
+  | DUG n _ => Some n
+  | _ => None
+  end.
+
+Definition undig {st tff A B} (i : instruction st tff A B) : Datatypes.option Datatypes.nat :=
+  let? o := unopcode i in undig_opcode o.
+
+Definition undug {st tff A B} (i : instruction st tff A B) : Datatypes.option Datatypes.nat :=
+  let? o := unopcode i in undug_opcode o.
+
+Lemma untype_inversion_undig {st tff A B um} (i : instruction st tff A B) n :
+  untyper.untype_instruction um i =
+  untyped_syntax.instruction_opcode (untyped_syntax.DIG n) ->
+  undig i = Some n.
+Proof.
+  intro H.
+  apply untype_inversion_dig in H.
+  repeat mytac.
+  reflexivity.
+Qed.
+
+Lemma untype_inversion_undug {st tff A B um} (i : instruction st tff A B) n :
+  untyper.untype_instruction um i =
+  untyped_syntax.instruction_opcode (untyped_syntax.DUG n) ->
+  undug i = Some n.
+Proof.
+  intro H.
+  apply untype_inversion_dug in H.
+  repeat mytac.
+  reflexivity.
+Qed.
+
+Definition digndugn_opt {st tff A D} (i : instruction_seq st tff A D) :
+  Datatypes.option (instruction_seq st tff A D) :=
+  let? existT _ _ (existT _ _ i1) := unseq_fst i in
+  let? existT _ _ (existT _ _ i23) := unseq_snd i in
+  let '(existT _ _ i1) := hide_ntf i1 in
+  let? existT _ _ (existT _ _ i2) := unseq_fst i23 in
+  let '(existT _ _ i2) := hide_ntf i2 in
+  let? existT _ _ (existT _ _ i3) := unseq_snd i23 in
+  let? n1 := undig i1 in
+  let? n2 := undug i2 in
+  if (n1 =? n2) then cast_instruction_seq_opt i3 else None.
+
+Inductive digndugn_rel {st tff} :
+  forall {A B} (i i' : instruction_seq st tff A B), Prop :=
+| DignDugn_intro {S1 S2 t B} (i : instruction_seq st tff (S1 +++ t ::: S2) B) :
+    digndugn_rel
+      (SEQ (@DIG st (List.length S1) S1 S2 t eq_refl)
+            (SEQ (@DUG st (List.length S1) S1 S2 t eq_refl) i)) i.
+
+Lemma digndugn_opt_digndugn {st tff A D} (i i' : instruction_seq st tff A D) :
+  digndugn_opt i = Some i' <->
+  digndugn_rel i i'.
+Proof.
+  split.
+  - unfold digndugn_opt.
+    intro H.
+    apply bind_some in H; destruct H as ((A1, (B1, i1)), (He1, H)).
+    apply bind_some in H; destruct H as ((A23, (B23, i23)), (He23, H)).
+    case_eq (hide_ntf i1); intros tff1 i1' Hi1'; rewrite Hi1' in H.
+    apply bind_some in H; destruct H as ((A2, (B2, i2)), (He2, H)).
+    case_eq (hide_ntf i2); intros tff2 i2' Hi2'; rewrite Hi2' in H.
+    apply bind_some in H; destruct H as ((A3, (B3, i3)), (He3, H)).
+
+    destruct i1'; try discriminate.
+    destruct o; try discriminate.
+    simpl in H.
+
+    destruct i2'; try discriminate.
+    destruct o; try discriminate.
+    simpl in H.
+
+    case_eq (n =? n0); intro Hn; rewrite Hn in H; [|discriminate].
+
+    destruct i; try discriminate.
+    destruct i23; try discriminate.
+    simpl in *.
+
+    repeat mytac.
+    match goal with | H : _ ::: _ +++ _ = _ ::: _ +++ _ |- _ => injection H end.
+    intros Happ Ht.
+    apply beq_nat_true in Hn.
+    symmetry in Hn.
+    apply untyper.app_length_inv in Happ; [|assumption].
+    repeat mytac.
+    constructor.
+  - intro H.
+    destruct H.
+    simpl.
+    unfold digndugn_opt; simpl.
+    rewrite Nat.eqb_refl.
+    apply cast_instruction_seq_same.
+Qed.
+
+Definition digndugn_aux {st tff A D} (i : instruction_seq st tff A D) :
+  instruction_seq st tff A D :=
+  opt_get (digndugn_opt i) i.
+
+Definition digndugn {st tff A B} (i : instruction_seq st tff A B) : instruction_seq st tff A B :=
+  visit_instruction_seq (@digndugn_aux) i.
+
+Lemma untype_digndugn : untype_fun_seq (@digndugn) (optimizer.digndugn).
+Proof.
+  unfold untype_fun_seq, digndugn, optimizer.digndugn.
+  apply untype_visit_instruction_seq; [| reflexivity].
+  intros st tff A D i; simpl.
+  unfold digndugn_aux.
+  unfold opt_get.
+  case_eq (digndugn_opt i).
+  - intros i' H.
+    rewrite digndugn_opt_digndugn in H.
+    destruct H.
+    simpl.
+    rewrite Nat.eqb_refl.
+    reflexivity.
+  - intro H.
+    unfold digndugn_opt in H.
+    case_eq (untyper.untype_instruction_seq untyper.untype_Optimized i);
+      try reflexivity.
+    intros ui1 ui23 Hi.
+    destruct ui1; try reflexivity.
+    destruct o; try reflexivity.
+    destruct ui23; try reflexivity.
+    destruct i0; try reflexivity.
+    destruct o; try reflexivity.
+    case_eq (n =? n0); intro Hn; try reflexivity.
+    exfalso.
+    generalize (untype_inversion_seq Hi).
+    intro Hiinv.
+    destruct Hiinv as [(Htff, (i', Hi')) | (B, (i1, (i23, Hi123)))].
+    * repeat mytac.
+      discriminate.
+    * subst i.
+      simpl in Hi.
+      injection Hi.
+      intros Hi23 Hi1.
+      generalize (untype_inversion_seq Hi23).
+      intros Hiinv.
+      destruct Hiinv as [(Htff, (i', Hi')) | (C, (i2, (i3, Hi23')))].
+      -- repeat mytac.
+         injection Hi23.
+         intros Hui23 Hi'.
+         apply untype_inversion_dug in Hi'.
+         repeat mytac.
+         discriminate.
+      -- repeat mytac.
+         injection Hi23.
+         intros Hi3 Hi2.
+         assert (undig i1 = Some n) as Hni1
+             by (eapply untype_inversion_undig; eassumption).
+         assert (undug i2 = Some n0) as Hni2
+             by (eapply untype_inversion_undug; eassumption).
+         simpl in H.
+         rewrite Hni1 in H.
+         rewrite Hni2 in H.
+         simpl in H.
+         rewrite Hn in H.
+         apply untype_inversion_dig in Hi1.
+         apply untype_inversion_dug in Hi2.
+         repeat mytac.
+         match goal with | H : _ ::: ?S1 +++ _ = _ ::: ?S2 +++ _ |- _ =>
+                           rename H into Hl end.
+         injection Hl; intros Happ Ht.
+         apply beq_nat_true in Hn.
+         symmetry in Hn.
+         apply untyper.app_length_inv in Happ; [|assumption].
+         repeat mytac.
+Qed.
+
+(* PUSH - DROP *)
+
+Definition unpush {st tff A B} (i : instruction st tff A B) : Datatypes.option Datatypes.unit :=
+  match i with
+  | PUSH _ _ => Some tt
+  | _ => None
+  end.
+
+Lemma untype_inversion_push {st tff A B um} (i : instruction st tff A B) a x :
+  untyper.untype_instruction um i =
+  untyped_syntax.PUSH a x ->
+  exists y (H : tff = false) (HB : B = a ::: A),
+    untyper.untype_data um y = x /\
+    eq_rec
+      _
+      (fun B => instruction st false A B)
+      (eq_rec _ (fun tff => instruction st tff A B) i _ H) _ HB
+    = PUSH a y.
+Proof.
+  destruct i; try discriminate.
+  simpl.
+  intro H.
+  injection H.
+  intros; subst; clear H.
+  eexists.
+  do 2 (exists eq_refl).
+  split; reflexivity.
+Qed.
+
+Definition undrop_opcode {st A B} (i : @opcode st A B) : Datatypes.option Datatypes.nat :=
+  match i with
+  | DROP n _ => Some n
+  | _ => None
+  end.
+
+Definition undrop {st tff A B} (i : instruction st tff A B) : Datatypes.option Datatypes.nat :=
+  let? o := unopcode i in undrop_opcode o.
+
+
+Lemma untype_inversion_drop {st tff A B um} (i : instruction st tff A B) n :
+  untyper.untype_instruction um i =
+  untyped_syntax.instruction_opcode (untyped_syntax.DROP n) ->
+  exists S1
+         (H : tff = false)
+         (HA : A = S1 +++ B)
+         (Hn : n = List.length S1),
+    eq_rec
+      _
+      (fun A => instruction st false A B)
+      (eq_rec _ (fun tff => instruction st tff A B) i _ H) _ HA
+    = Instruction_opcode (@DROP _ (List.length S1) S1 B eq_refl).
+Proof.
+  destruct i; try discriminate.
+  destruct o; try discriminate.
+  simpl.
+  intro H.
+  injection H.
+  intro; subst; clear H.
+  eexists.
+  do 3 (exists eq_refl).
+  reflexivity.
+Qed.
+
+Definition take_one_opt (A : stack_type) :
+  Datatypes.option (sigT (fun a : type =>
+                          sig (fun B : stack_type => A = a ::: B))) :=
+  match A with
+  | nil => None
+  | cons a A => Some (existT _ a (exist _ A eq_refl))
+  end.
+
+Fixpoint take_n_opt (A : stack_type) n :
+  Datatypes.option (sig (fun S1 : stack_type => List.length S1 = n)) :=
+  match n with
+  | 0 => Some (exist _ nil eq_refl)
+  | S n =>
+    let? existT _ a (exist _ B H) := take_one_opt A in
+    let? exist _ S1 H := take_n_opt B n in
+    Some (exist _ (a ::: S1) (f_equal S H))
+  end.
+
+Lemma take_n_opt_length S1 S2 : take_n_opt (S1 +++ S2) (Datatypes.length S1) =
+                                Some (exist _ S1 eq_refl).
+Proof.
+  induction S1; simpl.
+  - reflexivity.
+  - rewrite IHS1; reflexivity.
+Qed.
+
+Definition pushdrop_opt {st tff A D} (i : instruction_seq st tff A D) :
+  Datatypes.option (instruction_seq st tff A D) :=
+  let? existT _ _ (existT _ _ i1) := unseq_fst i in
+  let? existT _ _ (existT _ _ i23) := unseq_snd i in
+  let '(existT _ _ i1) := hide_ntf i1 in
+  let? existT _ _ (existT _ _ i2) := unseq_fst i23 in
+  let '(existT _ _ i2) := hide_ntf i2 in
+  let? existT _ B (existT _ _ i3) := unseq_snd i23 in
+  let? tt := unpush i1 in
+  let? n := undrop i2 in
+  match n with
+  | 0 => None
+  | 1 => cast_instruction_seq_opt i3
+  | S n =>
+    let? exist _ S1 H1 := take_n_opt A n in
+    cast_instruction_seq_opt (SEQ (@DROP st n S1 B H1) i3)
+  end.
+
+Inductive pushdrop_rel {st tff} :
+  forall {A B} (i i' : instruction_seq st tff A B), Prop :=
+| PushDrop_1 {A B t x} (i : instruction_seq st tff A B) :
+    pushdrop_rel
+      (SEQ (PUSH t x) (SEQ (@DROP _ 1 (cons t nil) A eq_refl) i)) i
+| PushDrop_S {t2 S1 S2 B t1 x} (i : instruction_seq st tff S2 B) :
+    pushdrop_rel
+      (SEQ (PUSH t1 x) (SEQ (@DROP _ (S (S (List.length S1))) (cons t1 (cons t2 S1)) S2 eq_refl) i))
+      (SEQ (@DROP _ (S (List.length S1)) (cons t2 S1) S2 eq_refl) i).
+
+Lemma pushdrop_opt_pushdrop {st tff A D} (i i' : instruction_seq st tff A D) :
+  pushdrop_opt i = Some i' <-> pushdrop_rel i i'.
+Proof.
+  split.
+  - unfold pushdrop_opt.
+    intro H.
+    apply bind_some in H; destruct H as ((A1, (B1, i1)), (He1, H)).
+    apply bind_some in H; destruct H as ((A23, (B23, i23)), (He23, H)).
+    case_eq (hide_ntf i1); intros tff1 i1' Hi1'; rewrite Hi1' in H.
+    apply bind_some in H; destruct H as ((A2, (B2, i2)), (He2, H)).
+    case_eq (hide_ntf i2); intros tff2 i2' Hi2'; rewrite Hi2' in H.
+    apply bind_some in H; destruct H as ((A3, (B3, i3)), (He3, H)).
+
+    destruct i1'; try discriminate.
+    simpl in H.
+
+    destruct i2'; try discriminate.
+    destruct o; try discriminate.
+    simpl in H.
+
+    destruct n as [|[|n]]; destruct A1 as [|t1[|t2 A1]]; try discriminate.
+    + destruct i; try discriminate.
+      destruct i23; try discriminate.
+      simpl in *.
+      repeat mytac.
+      constructor.
+    + destruct i; try discriminate.
+      destruct i23; try discriminate.
+      simpl in *.
+      injection e; intro.
+      repeat mytac.
+      rewrite take_n_opt_length in H1.
+      simpl in *.
+      repeat mytac.
+      simpl.
+      constructor.
+  - intro H.
+    destruct H.
+    + simpl.
+      unfold pushdrop_opt; simpl.
+      apply cast_instruction_seq_same.
+    + simpl.
+      unfold pushdrop_opt; simpl.
+      rewrite take_n_opt_length.
+      simpl.
+      apply cast_instruction_seq_same.
+Qed.
+
+Definition pushdrop_aux {st tff A B} (i : instruction_seq st tff A B)
+  : instruction_seq st tff A B :=
+  opt_get (pushdrop_opt i) i.
+
+Definition pushdrop {st tff A B} (i : instruction_seq st tff A B) :=
+  visit_instruction_seq (@pushdrop_aux) i.
+
+Lemma untype_pushdrop : untype_fun_seq (@pushdrop) (optimizer.push_drop).
+Proof.
+  unfold untype_fun_seq, pushdrop, optimizer.push_drop.
+  apply untype_visit_instruction_seq; [| reflexivity].
+  intros st tff A D i; simpl.
+  unfold pushdrop_aux.
+  unfold opt_get.
+  case_eq (pushdrop_opt i).
+  - intros i' H.
+    rewrite pushdrop_opt_pushdrop in H.
+    destruct H; reflexivity.
+  - intro H.
+    unfold pushdrop_opt in H.
+    case_eq (untyper.untype_instruction_seq untyper.untype_Optimized i);
+      try reflexivity.
+    intros ui1 ui23 Hi.
+    destruct ui1; try reflexivity.
+    destruct ui23; try reflexivity.
+    destruct i0; try reflexivity.
+    destruct o; try reflexivity.
+    destruct n as [|n]; try reflexivity.
+    exfalso.
+    generalize (untype_inversion_seq Hi).
+    intro Hiinv.
+    destruct Hiinv as [(Htff, (i', Hi')) | (B, (i1, (i23, Hi123)))].
+    * repeat mytac.
+      discriminate.
+    * subst i.
+      simpl in Hi.
+      injection Hi.
+      intros Hi23 Hi1.
+      generalize (untype_inversion_seq Hi23).
+      intros Hiinv.
+      destruct Hiinv as [(Htff, (i', Hi')) | (C, (i2, (i3, Hi23')))].
+      -- repeat mytac.
+         injection Hi23.
+         intros Hui23 Hi'.
+         apply untype_inversion_drop in Hi'.
+         repeat mytac.
+         discriminate.
+      -- repeat mytac.
+         injection Hi23.
+         intros Hi3 Hi2.
+         apply untype_inversion_push in Hi1.
+         apply untype_inversion_drop in Hi2.
+         repeat mytac.
+         match goal with H : S _ = Datatypes.length ?l |- _ =>
+                         rename l into B; rename H into HB end.
+         destruct B as [| a [| b B]]; [discriminate| |].
+         ++ simpl in *.
+            injection HB; intro.
+            repeat mytac.
+            simpl in H.
+            repeat mytac.
+         ++ simpl in *.
+            injection HB; intro.
+            repeat mytac.
+            simpl in H.
+            rewrite take_n_opt_length in H.
+            simpl in H.
+            repeat mytac.
+Qed.
+
+Definition cleanup {st tff A B} (i : instruction_seq st tff A B)
+  : instruction_seq st tff A B :=
+  pushdrop
+    (swapswap
+       (digndugn
+          (dig0dug0 i))).
+
+Lemma untype_cleanup : untype_fun_seq (@cleanup) (optimizer.cleanup).
+Proof.
+  intros st tff A B i.
+  unfold cleanup, optimizer.cleanup.
+  rewrite (@untype_pushdrop st tff A B); f_equal.
+  rewrite (@untype_swapswap st tff A B); f_equal.
+  rewrite (@untype_digndugn st tff A B); f_equal.
+  rewrite (@untype_dig0dug0 st tff A B); f_equal.
+Qed.
+
+
+Module Semantics_Preservation (C : semantics.ContractContext).
+  Module S := semantics.Semantics C.
+  Import S.
+
+  Definition same_semantics
+             (F : forall st tff A B, instruction_seq st tff A B ->
+                                     instruction_seq st tff A B)
+    :=
+      forall st tff env A B fuel i stA,
+        Bool.Is_true (error.success (eval_seq env i fuel stA)) ->
+        eval_seq env (F st tff A B i) fuel stA = eval_seq env i fuel stA.
+
+  Lemma eval_seq_SEQ st tff env A B C
+        (i1 : instruction st false A B)
+        (i2 : instruction_seq st tff B C) fuel SA :
+    eval_seq env (SEQ i1 i2) fuel SA =
+    let! SB := eval env i1 fuel SA in
+    eval_seq env i2 fuel SB.
+  Proof.
+    unfold eval_seq.
+    destruct fuel; reflexivity.
+  Qed.
+
+  Lemma eval_fail_and_seq :
+    (forall st A B (i : instruction st true A B)
+            fuel env stA, ~ Bool.Is_true (error.success (eval env i fuel stA))) *
+    (forall st A B (i : instruction_seq st true A B)
+            fuel env stA, ~ Bool.Is_true (error.success (eval_seq env i fuel stA))).
+  Proof.
+    apply tail_fail_induction_and_seq; intros; (destruct fuel as [|fuel]; [simpl; auto|]); simpl.
+    - destruct stA as (x, stA); simpl.
+      auto.
+    - destruct stA as (x, stA); simpl.
+      destruct (if_family_destruct f x); simpl; [apply H | apply H0].
+    - rewrite eval_seq_SEQ.
+      intro Hs; apply error.success_bind in Hs.
+      destruct Hs as (stB, (Hi1, Hs)).
+      apply H in Hs.
+      assumption.
+    - apply H.
+    - apply H.
+  Qed.
+
+  Lemma eval_fail st A B (i : instruction st true A B) fuel env stA :
+    ~ Bool.Is_true (error.success (eval env i fuel stA)).
+  Proof.
+    apply eval_fail_and_seq.
+  Qed.
+
+  Lemma eval_fail_seq st A B (i : instruction_seq st true A B) fuel env stA :
+    ~ Bool.Is_true (error.success (eval_seq env i fuel stA)).
+  Proof.
+    apply eval_fail_and_seq.
+  Qed.
+
+  Lemma same_semantics_visit_seq_aux F (HF : same_semantics F)
+        (HNOOP : forall st A, F st _ A A NOOP = NOOP) :
+    (forall st tff env A B fuel (i : instruction st tff A B) stA,
+        Bool.Is_true (error.success (eval env i fuel stA)) ->
+        eval env (visit_instruction F i) fuel stA = eval env i fuel stA) ->
+    same_semantics (@visit_instruction_seq F).
+  Proof.
+    intros Heval st tff env A B fuel i stA Hsucc.
+    induction i.
+    - simpl.
+      rewrite HNOOP.
+      reflexivity.
+    - simpl.
+      apply eval_fail in Hsucc.
+      contradiction.
+    - simpl.
+      rewrite eval_seq_SEQ in Hsucc.
+      apply error.success_bind in Hsucc.
+      destruct Hsucc as (stB, (Hi, Hsucc)).
+      transitivity
+        (eval_seq env (SEQ
+                         (visit_instruction F i)
+                         (visit_instruction_seq F i0)) fuel stA).
+      + apply HF.
+        rewrite eval_seq_SEQ.
+        specialize (IHi env stB Hsucc).
+        rewrite Heval; rewrite Hi; [|constructor].
+        simpl.
+        rewrite IHi.
+        assumption.
+      + do 2 rewrite eval_seq_SEQ.
+        rewrite Heval.
+        * rewrite Hi.
+          simpl.
+          apply IHi.
+          exact Hsucc.
+        * rewrite Hi.
+          simpl.
+          constructor.
+  Defined.
+
+  Fixpoint same_semantics_visit F (HF : same_semantics F) (HNOOP : forall st A, F st false A A NOOP = NOOP)
+           st tff env A B fuel (i : instruction st tff A B) stA {struct fuel} :
+    Bool.Is_true (error.success (eval env i fuel stA)) ->
+    eval env (visit_instruction F i) fuel stA =
+    eval env i fuel stA.
+  Proof.
+    specialize (same_semantics_visit_seq_aux F HF HNOOP (same_semantics_visit F HF HNOOP)).
+    unfold same_semantics.
+    intros Hseq.
+    destruct fuel as [|fuel]; [reflexivity|]; destruct i; try reflexivity.
+    + apply Hseq; try assumption.
+    + destruct stA as (x, SA);
+        simpl; destruct (if_family_destruct i x);
+          intro Hsucc; apply Hseq; exact Hsucc.
+    + destruct stA as (ab, SA); simpl; destruct (loop_family_destruct i ab) as [a|b];
+        intro Hsucc.
+      * apply error.success_bind in Hsucc.
+        destruct Hsucc as ((x, SA'), (Hret,Hsucc)).
+        unfold eval_seq in Hseq.
+        rewrite Hseq.
+        -- rewrite Hret; simpl.
+           unfold stack_type in Hret; rewrite Hret; simpl.
+           generalize (same_semantics_visit F HF HNOOP _ _ env _ _ fuel (LOOP_ i i0));
+             intro Hv.
+           simpl in Hv.
+           apply Hv.
+           assumption.
+        -- unfold stack_type in Hret.
+           rewrite Hret.
+           constructor.
+      * reflexivity.
+    + destruct stA as (x, SA); simpl.
+      destruct (iter_destruct (iter_elt_type collection i) collection (iter_variant_field collection i)) as [(a, y)|]; intro Hsucc.
+      * apply error.success_bind in Hsucc.
+        destruct Hsucc as (z, (Hret,Hsucc)).
+        unfold stack_type.
+        unfold eval_seq in Hseq.
+        rewrite Hseq.
+        -- generalize (same_semantics_visit F HF HNOOP _ _ env _ _ fuel (ITER i0));
+             intro Hv.
+           simpl in Hv.
+           unfold stack_type in Hret.
+           rewrite Hret.
+           simpl.
+           apply Hv.
+           assumption.
+        -- unfold stack_type in Hret.
+           rewrite Hret.
+           constructor.
+      * reflexivity.
+    + destruct stA as (x, SA); simpl.
+      destruct (map_destruct (map_in_type collection b i) b collection (map_out_collection_type collection b i) (map_variant_field collection b i) x) as [(a, y)|]; intro Hsucc.
+      * apply error.success_bind in Hsucc.
+        destruct Hsucc as ((b0, SB), (Hret,Hsucc)).
+        unfold eval_seq in Hseq.
+        rewrite Hseq.
+        -- generalize (same_semantics_visit F HF HNOOP self_type _ env _ _ fuel (MAP i0));
+             intro Hv.
+           simpl in Hv.
+           rewrite Hret.
+           unfold stack_type in Hret.
+           simpl.
+           simpl in Hret.
+           match goal with |- (let! (b1, SB0) := ?lhs in _ ) = _ =>
+                           replace lhs with (error.Return (b0, SB))
+           end.
+           simpl.
+           rewrite Hv.
+           ++ reflexivity.
+           ++ apply error.success_bind_arg in Hsucc.
+              assumption.
+        -- unfold stack_type in Hret.
+           match goal with |- (Bool.Is_true (error.success ?lhs)) =>
+                           replace lhs with (error.Return (b0, SB))
+           end.
+           constructor.
+      * reflexivity.
+    + simpl.
+      intro Hsucc.
+      destruct (stack_split stA) as (S1, S2).
+      unfold eval_seq in Hseq.
+      rewrite Hseq.
+      * reflexivity.
+      * unfold stack_type in Hsucc.
+        apply error.success_bind_arg in Hsucc.
+        assumption.
+  Qed.
+
+  Lemma same_semantics_visit_seq F (HF : same_semantics F) (HNOOP : forall st A, F st false A A NOOP = NOOP) :
+    same_semantics (@visit_instruction_seq F).
+  Proof.
+    apply same_semantics_visit_seq_aux; try assumption.
+    apply same_semantics_visit; assumption.
+  Qed.
+
+  Lemma same_semantics_opt F :
+    (forall st tff env A B (i i' : instruction_seq st tff A B) SA fuel,
+        F st tff A B i = Some i' ->
+        Bool.Is_true (error.success (eval_seq env i fuel SA)) ->
+        eval_seq env i' fuel SA = eval_seq env i fuel SA) ->
+    same_semantics (fun st tff A B (i : instruction_seq st tff A B) => opt_get (F st tff A B i) i).
+  Proof.
+    intros HF st tff env A B fuel i SA Hsucc.
+    case_eq (F st tff A B i).
+    - intros i' Hi'.
+      apply HF; assumption.
+    - intro; reflexivity.
+  Qed.
+
+  Lemma eval_Instruction_seq_aux st tff env A B (i : instruction_seq st tff A B) fuel stA :
+    Bool.Is_true (error.success (eval env (Instruction_seq i) fuel stA)) ->
+    eval env (Instruction_seq i) fuel stA =
+    eval_seq env i fuel stA.
+  Proof.
+    destruct fuel.
+    - contradiction.
+    - intro Hsucc.
+      change (eval_seq env i fuel stA = eval_seq env i (S fuel) stA).
+      apply eval_seq_deterministic_le.
+      + omega.
+      + assumption.
+  Qed.
+
+  Lemma eval_seq_instruction_app_aux st tff1 H1 tff2 env A B C
+        (i1 : instruction_seq st tff1 A B)
+        (i2 : instruction_seq st tff2 B C) fuel SA :
+    eval_seq env (instruction_app_aux i1 H1 i2) fuel SA =
+    let! SB := eval_seq env i1 fuel SA in
+    eval_seq env i2 fuel SB.
+  Proof.
+    induction i1; simpl.
+    - reflexivity.
+    - discriminate.
+    - unfold eval_seq.
+      simpl.
+      destruct (eval env i fuel SA); simpl.
+      + reflexivity.
+      + apply IHi1.
+  Qed.
+
+  Lemma eval_seq_instruction_app st tff env A B C
+        (i1 : instruction_seq st false A B)
+        (i2 : instruction_seq st tff B C) fuel SA :
+    eval_seq env (i1;;;i2) fuel SA =
+    let! SB := eval_seq env i1 fuel SA in
+    eval_seq env i2 fuel SB.
+  Proof.
+    apply eval_seq_instruction_app_aux.
+  Qed.
+
+  Lemma eval_Instruction_seq self_type tff env fuel A B C
+        (i1 : instruction_seq self_type false A B)
+        (i2 : instruction_seq self_type tff B C)
+        stA:
+    Bool.Is_true (error.success (eval_seq env (SEQ (Instruction_seq i1) i2) fuel stA)) ->
+    eval_seq env (i1;;; i2) fuel stA =
+    eval_seq env (SEQ (Instruction_seq i1) i2) fuel stA.
+  Proof.
+    intro Hsucc.
+    rewrite eval_seq_instruction_app.
+    rewrite eval_seq_SEQ.
+    rewrite eval_Instruction_seq_aux.
+    - reflexivity.
+    - rewrite eval_seq_SEQ in Hsucc.
+      apply error.success_bind_arg in Hsucc.
+      assumption.
+  Qed.
+
+  Lemma same_semantics_dig0dug0 :
+    same_semantics (@dig0dug0).
+  Proof.
+    apply same_semantics_visit_seq.
+    - apply same_semantics_opt.
+      intros st tff env A B i i' stA fuel HS Hsucc.
+      apply dig0dug0_opt_dig0dug0 in HS.
+      destruct HS.
+      + apply eval_fail_seq in Hsucc.
+        contradiction.
+      + apply eval_Instruction_seq.
+        assumption.
+      + rewrite eval_seq_instruction_app.
+        rewrite eval_seq_SEQ.
+        f_equal.
+        unfold eval_seq in Hsucc.
+        apply error.success_bind in Hsucc.
+        destruct Hsucc as (stB, (HDIP, _)).
+        destruct fuel; [simpl in HDIP; discriminate|].
+        simpl.
+        simpl in HDIP.
+        apply error.bind_eq_return in HDIP.
+        destruct HDIP as (stB', (Hi1, HstB')).
+        apply error.unreturn in HstB'.
+        subst stB'.
+        rewrite Hi1.
+        simpl.
+        rewrite <- Hi1.
+        symmetry.
+        apply eval_seq_deterministic_le; [omega|].
+        unfold eval_seq.
+        unfold stack_type in Hi1.
+        rewrite Hi1.
+        constructor.
+      + rewrite eval_seq_SEQ.
+        destruct fuel; [simpl in Hsucc; contradiction|].
+        reflexivity.
+      + rewrite eval_seq_SEQ.
+        destruct fuel; [simpl in Hsucc; contradiction|].
+        destruct stA; reflexivity.
+      + rewrite eval_seq_SEQ.
+        destruct fuel; [simpl in Hsucc; contradiction|].
+        destruct stA; reflexivity.
+      + rewrite eval_seq_SEQ.
+        destruct fuel; [simpl in Hsucc; contradiction|].
+        destruct stA as (x, (y, stA)); reflexivity.
+      + rewrite eval_seq_SEQ.
+        destruct fuel; [simpl in Hsucc; contradiction|].
+        destruct stA as (x, (y, stA)); reflexivity.
+    - reflexivity.
+  Qed.
+
+
+  Lemma same_semantics_swapswap :
+    same_semantics (@swapswap).
+  Proof.
+    apply same_semantics_visit_seq.
+    - apply same_semantics_opt.
+      intros st tff env A D i i' stA fuel HS Hsucc.
+      apply swapswap_opt_swapswap in HS.
+      destruct HS.
+      destruct fuel as [|fuel]; [contradiction|].
+      destruct stA as (x, (y, stA)).
+      rewrite eval_seq_SEQ.
+      simpl.
+      rewrite eval_seq_SEQ.
+      simpl.
+      reflexivity.
+    - reflexivity.
+  Qed.
+
+  Lemma stack_app_split (S1 S2 : Datatypes.list type) (s1 : stack S1) (s2 : stack S2) sA :
+    stack_split sA = (s1, s2) <-> sA = stack_app s1 s2.
+  Proof.
+    generalize s2; clear s2.
+    induction S1; intro s2.
+    - simpl.
+      simpl in s1.
+      destruct s1.
+      split; congruence.
+    - simpl.
+      simpl in s1.
+      destruct s1 as (x, s1).
+      simpl in sA.
+      destruct sA as (y, sA).
+      case_eq (stack_split sA).
+      intros s1' s2' HsA.
+      split.
+      + rewrite IHS1 in HsA.
+        congruence.
+      + intro H; injection H; intros.
+        subst y.
+        rewrite <- IHS1 in H0.
+        congruence.
+  Qed.
+
+  Lemma same_semantics_digndugn :
+    same_semantics (@digndugn).
+  Proof.
+    apply same_semantics_visit_seq.
+    - apply same_semantics_opt.
+      intros st tff env A D i i' stA fuel HS Hsucc.
+      apply digndugn_opt_digndugn in HS.
+      destruct HS.
+      + destruct fuel as [|fuel]; [contradiction|].
+        rewrite eval_seq_SEQ.
+        simpl.
+        rewrite eval_seq_SEQ.
+        simpl.
+        unfold stack_dig, stack_dug.
+        case_eq (stack_split stA).
+        intros s1 s2 HS12.
+        destruct s2 as (x, s2).
+        assert (stack_split (stack_app s1 s2) = (s1, s2)) as H.
+        * rewrite stack_app_split.
+          reflexivity.
+        * rewrite H.
+          rewrite stack_app_split in HS12.
+          congruence.
+    - reflexivity.
+  Qed.
+
+  Lemma same_semantics_push_drop :
+    same_semantics (@pushdrop).
+  Proof.
+    apply same_semantics_visit_seq.
+    - apply same_semantics_opt.
+      intros st tff env A D i i' stA fuel HS Hsucc.
+      apply pushdrop_opt_pushdrop in HS.
+      destruct HS.
+      + destruct fuel as [|fuel]; [contradiction|].
+        rewrite eval_seq_SEQ.
+        simpl.
+        rewrite eval_seq_SEQ.
+        simpl.
+        reflexivity.
+      + destruct fuel as [|fuel]; [contradiction|].
+        rewrite eval_seq_SEQ.
+        simpl.
+        rewrite eval_seq_SEQ.
+        simpl.
+        rewrite eval_seq_SEQ.
+        simpl.
+        destruct stA as (y, stA).
+        case_eq (stack_split stA).
+        reflexivity.
+    - reflexivity.
+  Qed.
+
+  Lemma same_semantics_compose F G :
+    same_semantics F ->
+    same_semantics G ->
+    same_semantics (fun st tff A B i => F st tff A B (G st tff A B i)).
+  Proof.
+    intros HF HG.
+    unfold same_semantics.
+    intros.
+    rewrite HF.
+    - rewrite HG.
+      + reflexivity.
+      + assumption.
+    - rewrite HG; assumption.
+  Qed.
+
+  Lemma same_semantics_cleanup :
+    same_semantics (@cleanup).
+  Proof.
+    unfold cleanup.
+    apply same_semantics_compose; [exact same_semantics_push_drop|].
+    apply same_semantics_compose; [exact same_semantics_swapswap|].
+    apply same_semantics_compose; [exact same_semantics_digndugn|].
+    exact same_semantics_dig0dug0.
+  Qed.
+
+  Definition typecheck_and_eval_seq
+             (i : untyped_syntax.instruction_seq)
+             A B (sA : stack A)
+             self_type env fuel : error.M (stack B) :=
+    let! existT _ tff i' :=
+       typer.type_check_instruction_seq
+         (self_type := self_type)
+         (typer.type_instruction_seq typer.Optimized)
+         i A B in
+    eval_seq env i' fuel sA.
+
+  (* If the untyped instruction sequence i can be typechecked from
+     stack type A to stack type B and then run successfully on stack
+     sA, then (optimizer.optimize i) can also be typechecked from
+     stack type A to stack type B and run successfully on stack sA
+     yielding the same result. *)
+
+  Theorem optimize_correct :
+    forall i A B sA self_type env fuel,
+      let e := typecheck_and_eval_seq i A B sA self_type env fuel in
+      Bool.Is_true (error.success e) ->
+      typecheck_and_eval_seq (optimizer.optimize i) A B sA self_type env fuel = e.
+  Proof.
+    intros ui A B sA self_type env fuel.
+    unfold typecheck_and_eval_seq.
+    intro Hsucc.
+    apply error.success_bind in Hsucc.
+    destruct Hsucc as ((tff, i), (Hret, Hsucc)).
+    rewrite Hret.
+    simpl.
+    unfold typer.type_check_instruction_seq in Hret.
+    apply error.bind_eq_return in Hret.
+    destruct Hret as (t, (Ht, Hret)).
+    apply untyper.type_untype_seq in Ht.
+    destruct t.
+    - subst ui.
+      unfold typer.instruction_seq_cast_range, typer.instruction_seq_cast in Hret.
+      rewrite untyper.stype_dec_same in Hret.
+      destruct (stype_dec B0 B); [|discriminate].
+      simpl in Hret.
+      apply error.unreturn in Hret.
+      repeat mytac.
+      rewrite <- (untype_cleanup).
+      unfold typer.type_check_instruction_seq.
+      simpl in *.
+      rewrite untyper.untype_type_instruction_seq.
+      simpl.
+      unfold typer.instruction_seq_cast_range.
+      rewrite untyper.instruction_seq_cast_same.
+      simpl.
+      apply same_semantics_cleanup.
+      assumption.
+    - apply error.unreturn in Hret.
+      repeat mytac.
+      simpl in Hsucc.
+      apply eval_fail_seq in Hsucc.
+      contradiction.
+  Qed.
+
+End Semantics_Preservation.
